src/aux.lean
@@ -1,3 +1,5 @@
+import data.vector
+
 namespace list_aux
 
 lemma list_length_neq_zero {α} {l : list α} (h : ¬(l.length = 0)) : ∃ x xs, l = (x :: xs) := begin
@@ -40,3 +42,122 @@ namespace set_aux
 lemma union_no_mem_left {α : Type} {a : α} {b c : set α} (h : a ∉ b ∪ c) : a ∉ b := sorry
 
 end set_aux
+
+namespace vector
+
+protected def mem {α : Type} {n : ℕ} : α → vector α n → Prop
+| a v := a ∈ v.to_list
+
+instance {α : Type} {n : ℕ} : has_mem α (vector α n) :=
+⟨vector.mem⟩
+
+set_option trace.eqn_compiler.elim_match true
+
+lemma nat_le_zero {n : ℕ} : n < 0 → false := by sorry
+
+-- lemma da {α} {n} {tl : list α} {a hd : α} {h : tl.length = n} : a ∈ (⟨tl, h⟩ : vector α n) → a ∈ (⟨hd :: tl, h⟩ : vector α n)
+
+lemma contains_nth {α : Type} {n : ℕ} {v : vector α n} {i : fin n} : (v.nth i) ∈ v := begin
+    induction n,
+    case nat.zero {
+        cases i,
+        apply false.elim,
+        apply nat_le_zero i_is_lt,
+    },
+    case nat.succ {
+        --rw ← cons_head_tail v,
+        cases i,
+        cases v,
+        cases v_val,
+        case list.nil {
+            sorry -- contr
+        },
+        case list.cons {
+            cases i_val,
+            case nat.zero {
+                rw nth,
+                simp, -- should be trivial but how to unfold ∈?
+                sorry,
+            },
+            case nat.succ {
+                rw nth,
+                simp,
+
+            }
+        }
+    }
+end
+
+--     have : ¬(0 < 0) := by sorry,
+--     cases i,
+--     induction i_val,
+--     case nat.zero {
+--         cases n,
+--         case nat.zero {
+--             contradiction,
+--         },
+--         case nat.succ {
+--             cases v,
+--             cases v_val,
+--             case list.nil {
+--                 rw ← v_property at i_is_lt,
+--                 simp at i_is_lt,
+--                 contradiction,
+--             },
+--             case list.cons {
+--                 rw nth,
+--                 simp,
+--                 sorry, -- should be trivial but how to unfold ∈?
+--             },
+--         }
+--     },
+--     case nat.succ {
+--         -- index is either i_val_n + 1 or below
+--         cases v,
+--         cases v_val,
+--         case list.nil {
+--             sorry -- proof by contr.
+--         },
+--         case list.cons {
+--             rw nth,
+--             rw list.nth_le,
+--             have : i_val_n < n := by sorry,
+--             specialize i_val_ih this,
+--             rw nth at i_val_ih,
+--             rw list.nth_le at i_val_ih,
+--         }
+--     }
+-- end
+
+-- begin
+--   have h_hdtl : ∃ x xs, s.threads = (x :: xs) := begin
+--     apply list_aux.list_length_neq_zero,
+--     apply nat_aux.lt_neq_zeor t,
+--     assumption,
+--   end,
+--   cases h_hdtl with ts' h_hdtl,
+--   cases h_hdtl with tail heq,
+--   induction t,
+--   case nat.zero {
+--     have : ts = ts' := begin
+--       rw ← h,
+--       rw heq at hl,
+--       rw th,
+--       sorry,
+--     end,
+--     rw this,
+--     rw heq,
+--     simp,
+--   },
+--   case nat.succ {
+--     by_cases hleq : t_n < list.length (s.threads),
+--     {
+--       apply t_ih hleq,
+--       assumption,
+--     }, {
+
+--     }
+--   }
+-- end
+
+end vector
